stlc updates

src/cli.rs
@@ -3,7 +3,7 @@ use std::{env, path::PathBuf};
 use anyhow::Context;
 use clap::{Parser, Subcommand};
 
-use etna::commands::{self, experiment::visualize::MetricType, store::query::QueryOption};
+use etna::commands::{self, experiment::visualize::{MetricType, VisualizationType}, store::query::QueryOption};
 use fern::colors::ColoredLevelConfig;
 
 fn main() -> anyhow::Result<()> {
@@ -76,7 +76,7 @@ pub(crate) fn run() -> anyhow::Result<()> {
                         name,
                         show_all,
                     } => commands::experiment::show::invoke(hash, name, show_all),
-            ExperimentCommand::Visualize { name, figure, tests, groupby, aggby, metric, buckets } => commands::experiment::visualize::invoke(name, figure, tests, groupby, aggby, metric, buckets),
+            ExperimentCommand::Visualize { name, figure, tests, groupby, aggby, metric, buckets, visualization_type } => commands::experiment::visualize::invoke(name, figure, tests, groupby, aggby, metric, buckets, visualization_type),
         },
         Command::Workload(wl) => match wl {
             WorkloadCommand::AddWorkload {
@@ -198,6 +198,11 @@ enum ExperimentCommand {
         /// Buckets to use for the visualization
         #[clap(short, long, value_parser, num_args = 1.., value_delimiter = ' ', default_values_t = vec![0.1, 1.0, 10.0, 60.0])]
         buckets: Vec<f64>,
+        /// Type of visualization
+        /// [default: "bucket"]
+        /// [possible_values(line, bar, bucket)]
+        #[clap(short, long, default_value_t = VisualizationType::Bucket)]
+        visualization_type: VisualizationType,
     },
 }
 #[derive(Debug, Subcommand)]
