workloads/Racket/RBT/Strategies/RackcheckBespoke.rkt
@@ -10,61 +10,63 @@
 
 (provide (all-defined-out))
 
+(define truthy?
+  (λ (x) (or (equal? x #t) (equal? x (just #t)))))
 
 #| Validity Properties |#
 
 (define test_prop_InsertValid
     (property insertValid ([t bespoke] [k gen:natural] [v gen:natural])
-        (equal? (prop_InsertValid t k v) (just #t)))
+        (truthy? (prop_InsertValid t k v)))
 )
 
 (define test_prop_DeleteValid
     (property deleteValid ([t bespoke] [k gen:natural])
-        (equal? (prop_DeleteValid t k) (just #t)))
+        (truthy? (prop_DeleteValid t k)))
 )
 
 #| Post-condition Properties |#
 
 (define test_prop_InsertPost
     (property insertPost ([t bespoke] [k1 gen:natural] [k2 gen:natural] [v gen:natural])
-        (equal? (prop_InsertPost t k1 k2 v) (just #t)))
+        (truthy? (prop_InsertPost t k1 k2 v)))
 )
 
 (define test_prop_DeletePost
     (property deletePost ([t bespoke] [k1 gen:natural] [k2 gen:natural])
-        (equal? (prop_DeletePost t k1 k2) (just #t)))
+        (truthy? (prop_DeletePost t k1 k2)))
 )
 
 #| Model-based Properties |#
 
 (define test_prop_InsertModel
     (property insertModel ([t bespoke] [k gen:natural] [v gen:natural])
-        (equal? (prop_InsertModel t k v) (just #t)))
+        (truthy? (prop_InsertModel t k v)))
 )
 
 (define test_prop_DeleteModel
     (property deleteModel ([t bespoke] [k gen:natural])
-        (equal? (prop_DeleteModel t k) (just #t)))
+        (truthy? (prop_DeleteModel t k)))
 )
 
 #| Metamorphic Properties |#
 
 (define test_prop_InsertInsert
     (property insertInsert ([t bespoke] [k1 gen:natural] [k2 gen:natural] [v1 gen:natural] [v2 gen:natural])
-        (equal? (prop_InsertInsert t k1 k2 v1 v2) (just #t)))
+        (truthy? (prop_InsertInsert t k1 k2 v1 v2)))
 )
 
 (define test_prop_InsertDelete
     (property insertDelete ([t bespoke] [k1 gen:natural] [k2 gen:natural] [v gen:natural])
-        (equal? (prop_InsertDelete t k1 k2 v) (just #t)))
+        (truthy? (prop_InsertDelete t k1 k2 v)))
 )
 
 (define test_prop_DeleteInsert
     (property deleteInsert ([t bespoke] [k1 gen:natural] [k2 gen:natural] [v gen:natural])
-        (equal? (prop_DeleteInsert t k1 k2 v) (just #t)))
+        (truthy? (prop_DeleteInsert t k1 k2 v)))
 )
 
 (define test_prop_DeleteDelete
     (property deleteDelete ([t bespoke] [k1 gen:natural] [k2 gen:natural])
-        (equal? (prop_DeleteDelete t k1 k2) (just #t)))
+        (truthy? (prop_DeleteDelete t k1 k2)))
 )
