workloads/Rust/stlc/src/lib.rs
@@ -3,4 +3,4 @@
 pub mod implementation;
 pub mod spec;
 pub mod strategies;
-
+pub mod parser;
