workloads/Rust/stlc/src/main_serialized.rs
@@ -1,9 +1,94 @@
-use std::path::Path;
+use std::{path::Path, process::ExitCode};
 
-use stlc::{spec, strategies::bespoke::ExprOpt};
-use trace::init_depth_var;
+use etna_rs_utils::{SamplingResult, Status};
+use stlc::{parser, spec, strategies::bespoke::ExprOpt};
 
-fn main() {
+fn sample(property: String, tests: &str) -> SamplingResult {
+    let mut discarded = 0;
+    let mut passed = 0;
+    match property.as_str() {
+        "SinglePreserve" => {
+            let Ok(tests) = parser::parse(&tests) else {
+                return SamplingResult {
+                    property,
+                    status: Status::Aborted("failed to parse tests".to_string()),
+                    tests: 0,
+                    passed,
+                    discarded,
+                };
+            };
+
+            for e in tests.into_iter() {
+                match spec::prop_single_preserve(ExprOpt(Some(e.clone()))) {
+                    None => {
+                        discarded += 1;
+                    }
+                    Some(true) => {
+                        passed += 1;
+                    }
+                    Some(false) => {
+                        return SamplingResult {
+                            property,
+                            status: Status::FoundBug(format!("{}", e)),
+                            tests: passed + discarded,
+                            passed,
+                            discarded,
+                        };
+                    }
+                }
+            }
+        }
+        "MultiPreserve" => {
+            let Ok(tests) = parser::parse(&tests) else {
+                return SamplingResult {
+                    property,
+                    status: Status::Aborted("failed to parse tests".to_string()),
+                    tests: 0,
+                    passed,
+                    discarded,
+                };
+            };
+
+            for e in tests.into_iter() {
+                match spec::prop_multi_preserve(ExprOpt(Some(e.clone()))) {
+                    None => {
+                        discarded += 1;
+                    }
+                    Some(true) => {
+                        passed += 1;
+                    }
+                    Some(false) => {
+                        return SamplingResult {
+                            property,
+                            status: Status::FoundBug(format!("{}", e)),
+                            tests: passed + discarded,
+                            passed,
+                            discarded,
+                        };
+                    }
+                }
+            }
+        }
+        _ => {
+            return SamplingResult {
+                status: Status::Aborted(format!("Unknown property: {}", property)),
+                property,
+                tests: 0,
+                passed,
+                discarded,
+            };
+        }
+    }
+    return SamplingResult {
+        property,
+        status: Status::Finished,
+        tests: passed + discarded,
+        passed,
+        discarded,
+    };
+}
+
+fn main() -> ExitCode {
     let args = std::env::args().collect::<Vec<_>>();
     if args.len() < 3 {
         eprintln!("Usage: {} <tests> <property>", args[0]);
@@ -11,7 +96,7 @@ fn main() {
         eprintln!(
             "For available properties, check https://github.com/alpaylan/etna-cli/blob/main/docs/workloads/stlc.md"
         );
-        return;
+        return ExitCode::FAILURE;
     }
     let tests = args[1].as_str();
     let property = args[2].as_str();
@@ -22,68 +107,12 @@ fn main() {
         tests.to_string()
     };
 
-    match property {
-        "SinglePreserve" => {
-            let tests: Vec<ExprOpt> = serde_lexpr::from_str(&tests).unwrap_or_else(|_| {
-                eprintln!("Failed to parse tests: '{}'", tests);
-                return vec![];
-            });
-            println!("Running SinglePreserve property tests...");
+    let result = sample(property.to_string(), &tests);
 
-            for (i, e) in tests.into_iter().enumerate() {
-                println!("Test {}: {:?}", i, e);
-                match spec::prop_single_preserve(e.clone()) {
-                    None => {
-                        eprintln!(
-                            "Test {} discarded for SinglePreserve: ({})",
-                            i,
-                            serde_lexpr::to_string(&e).unwrap_or_else(|_| {
-                                "failed to serialize STLC expression".to_string()
-                            })
-                        );
-                    }
-                    Some(true) => {
-                        println!(
-                            "Test {} passed for SinglePreserve: ({})",
-                            i,
-                            serde_lexpr::to_string(&e).unwrap_or_else(|_| {
-                                "failed to serialize STLC expression".to_string()
-                            })
-                        );
-                    }
-                    Some(false) => {
-                        eprintln!(
-                            "Test {} failed for SinglePreserve: ({})",
-                            i,
-                            serde_lexpr::to_string(&e).unwrap_or_else(|_| {
-                                "failed to serialize STLC expression".to_string()
-                            })
-                        );
-                        break;
-                    }
-                }
-            }
-        }
-        "MultiPreserve" => {
-            let tests: Vec<ExprOpt> = serde_lexpr::from_str(&tests).unwrap_or_else(|_| {
-                eprintln!("Failed to parse tests: '{}'", tests);
-                return vec![];
-            });
+    println!("{}", result);
 
-            for (i, e) in tests.into_iter().enumerate() {
-                if !spec::prop_multi_preserve(e.clone()).unwrap_or(true) {
-                    eprintln!(
-                        "Test {} failed for MultiPreserve: ({})",
-                        i,
-                        serde_lexpr::to_string(&e)
-                            .unwrap_or_else(|_| "failed to serialize STLC expression".to_string())
-                    );
-                }
-            }
-        }
-
-        _ => {
-            eprintln!("Unknown property: {}", property);
-        }
+    match result.status {
+        Status::Finished => ExitCode::SUCCESS,
+        Status::FoundBug(_) | Status::Aborted(_) => ExitCode::FAILURE,
     }
 }
