workloads/Rocq/STLC/Runners/BespokeGenerator_sampler.v
@@ -1,0 +1,79 @@
+From QuickChick Require Import QuickChick.
+
+Set Warnings "-extraction-opaque-accessed,-extraction".
+
+From STLC Require Import Impl Spec BespokeGeneration.
+
+Local Open Scope string_scope.
+
+#[local] Instance showTimedResult {A: Type} `{Show A} : Show (@TimedResult A) := {|
+  show result := 
+    let '(TResult result time start ending) := result in
+     "{ ""time"": """ ++ show time ++ """, ""value"": """ ++ show result ++ """ }"
+|}.
+
+
+Definition showTimedResultList {A: Type} `{Show A} (results : list (@TimedResult A)) : string :=
+  "[" ++ String.concat ", " (List.map (fun r => show r) results) ++ "]".
+
+Inductive Args1 {A : Type} : Type :=
+  | Args1Mk : A -> Args1.
+
+#[local] Instance ShowArgs1 {A} `{Show A} : Show (@Args1 A) :=
+  { show := fun '(Args1Mk a) => show a }.
+
+#[local] Instance ShowExprOpt : Show (option Expr) :=
+  { show := fun e =>
+    match e with
+    | Some e' => show e'
+    | None => ""
+    end
+  }.
+
+Definition sample_SinglePreserve    :=
+  bindGen gSized (fun (e: option Expr)  =>
+  ret (Args1Mk e))
+.
+
+Definition qctest_sample_SinglePreserve := (fun num_tests: nat => print_extracted_coq_string (showTimedResultList (quickSample (updMaxDiscard (updMaxSuccess (updAnalysis stdArgs true) num_tests) num_tests) sample_SinglePreserve))).
+
+
+Definition sample_MultiPreserve    :=
+    bindGen gSized (fun (e: option Expr)  =>
+    ret (Args1Mk e))
+.
+
+Definition qctest_sample_MultiPreserve := (fun num_tests: nat => print_extracted_coq_string (showTimedResultList (quickSample (updMaxDiscard (updMaxSuccess (updAnalysis stdArgs true) num_tests) num_tests) sample_MultiPreserve))).
+
+
+Parameter OCamlString : Type.
+Extract Constant OCamlString => "string".
+
+Axiom test_map : list (OCamlString * (nat -> unit)).
+Extract Constant test_map => "[
+    (""SinglePreserve"", qctest_sample_SinglePreserve);
+    (""MultiPreserve"", qctest_sample_MultiPreserve);
+]".
+
+Axiom qctest_map : OCamlString -> nat -> unit.
+Extract Constant qctest_map => "
+fun property num_tests ->
+  let test = List.assoc property test_map in
+  test num_tests
+
+
+let () =
+  let args = Sys.argv in
+  if Array.length args <> 3 then
+    Printf.eprintf ""Usage: %s <property> <#tests>\n"" args.(0)
+  else
+    let property = args.(1) in
+    let num_tests = int_of_string args.(2) in
+    if not (List.mem_assoc property test_map) then
+      Printf.eprintf ""Unknown test name: %s\n"" property
+    else
+      qctest_map property num_tests
+".
+
+
+Extraction "BespokeGenerator_sampler.ml" test_map qctest_map qctest_sample_SinglePreserve qctest_sample_MultiPreserve.
